Change the compiler to target the subst-semantics

compiler/backend/pure_to_thunkScript.sml
@@ -1,45 +1,17 @@
 (*
-   A compiler from pureLang to thunkLang.
+   A compiler from pureLang to the substitution-based version of
+   thunkLang.
 
-   - Moves from a substitution-based (probably) call-by-need semantics
-     to an environment-based (probably) call-by-value semantics with
-     explicit Delay/Force expressions.
  *)
 
 open HolKernel Parse boolLib bossLib term_tactic monadsyntax;
 open listTheory rich_listTheory;
-open pure_expTheory thunkLangTheory;
+open pure_expTheory thunkLang_substTheory;
 
 val _ = new_theory "pure_to_thunk";
 
-(*
- * The source language is call-by-need and the target language is call-by-value.
- * The difference between the two styles becomes apparent in value bindings
- * (letrecs) and function application:
- * - The compiler assumes that all Letrec expressions are already transformed
- *   into lambdas. That is, all non-functional declarations such as “let v = 8”
- *   have been turned into “let v = λu. 8” and all references to “v” have been
- *   changed into “v ()”.
- * - At function application sites, the compiler wraps the argument with the
- *   “Delay” constructor (essentially turning it into a thunk).
- * - The compiler inserts “Force” constructors <in some places> TODO
- * Other differences:
- * - If is a primitive operation (i.e. a “Prim”) in pureLang, but has become
- *   an expression in thunkLang.
- *)
-
-(* TODO
- * pure_exp theorem.
- *)
-Theorem exp_size_MEM:
-  MEM x xs ⇒ exp_size x < exp3_size xs
-Proof
-  Induct_on ‘xs’ \\ rw []
-  \\ fs [pure_expTheory.exp_size_def]
-QED
-
 Definition compile_exp_def:
-  compile_exp (Var n : pure_exp$exp) = thunkLang$Var n ∧
+  compile_exp (Var n : pure_exp$exp) = thunkLang_subst$Var n ∧
   compile_exp (Prim op xs) =
     (if op = If ∧ LENGTH xs = 3 then
        If (compile_exp (EL 0 xs))
@@ -50,19 +22,56 @@ Definition compile_exp_def:
   compile_exp (App x y) = App (compile_exp x) (Delay (compile_exp y)) ∧
   compile_exp (Lam v x) = Lam v (compile_exp x) ∧
   compile_exp (Letrec funs x) =
-    Letrec (MAP (λ(fn, x). case x of Lam v bod =>
-                             (fn, v, compile_exp bod)) funs)
+    Letrec (MAP (λ(fn, x). case x of
+                             Lam v bod => (fn, v, compile_exp bod)
+                           | _ => ("", "", Var "")) funs)
            (compile_exp x)
 Termination
   WF_REL_TAC ‘measure exp_size’
   \\ dsimp [pure_expTheory.exp_size_def, LENGTH_EQ_NUM_compute]
   \\ rw []
-  >- (
-    rename1 ‘MEM _ xs’
-    \\ Induct_on ‘xs’ \\ rw []
-    \\ fs [pure_expTheory.exp_size_def])
-  \\ drule exp_size_MEM \\ fs []
+  \\ (drule (CONJUNCT2 exp_size_lemma) ORELSE
+      drule (CONJUNCT1 exp_size_lemma))
+  \\ simp [pure_expTheory.exp_size_def]
 End
+
+Definition No_Value_def:
+  No_Value (Var v) = T ∧
+  No_Value (Prim op xs) = EVERY No_Value xs ∧
+  No_Value (App x y) = (No_Value x ∧ No_Value y) ∧
+  No_Value (Lam v x) = No_Value x ∧
+  No_Value (Letrec f x) = (EVERY No_Value (MAP (SND o SND) f) ∧ No_Value x) ∧
+  No_Value (If x y z) = (No_Value x ∧ No_Value y ∧ No_Value z) ∧
+  No_Value (Delay x) = No_Value x ∧
+  No_Value (Force x) = No_Value x ∧
+  No_Value (Value v) = F
+Termination
+  WF_REL_TAC ‘measure exp_size’ \\ rw []
+  \\ fs [pairTheory.LAMBDA_PROD, MEM_MAP, pairTheory.EXISTS_PROD]
+  \\ rename1 ‘MEM _ xs’
+  \\ Induct_on ‘xs’ \\ rw []
+  \\ fs [thunkLang_substTheory.exp_size_def]
+End
+
+Theorem compile_exp_No_Value:
+  ∀x. No_Value (compile_exp x)
+Proof
+  ho_match_mp_tac compile_exp_ind
+  \\ simp [compile_exp_def, No_Value_def]
+  \\ rpt conj_tac
+  \\ rpt gen_tac
+  \\ strip_tac
+  >- (
+    rw [No_Value_def, EVERY_MAP, EVERY_MEM]
+    \\ fs [])
+  >- (
+    simp [EVERY_MEM]
+    \\ simp [MAP_MAP_o, MEM_MAP, pairTheory.EXISTS_PROD, PULL_EXISTS]
+    \\ rpt gen_tac
+    \\ CASE_TAC \\ fs [No_Value_def]
+    \\ strip_tac
+    \\ res_tac)
+QED
 
 val _ = export_theory ();
 
